# 信号处理原理 第 4 次作业 #

李祥泽 2018011331

## 1 ##

求 $f(t)=e^{-at}\ ,a>0,t>0$ 的傅里叶变换. 

$$
\begin{align}
F(j\omega) &= \mathcal{F}[f(t)] \\
&= \int_0^\infty{f(t)e^{-j\omega t}\text{d}t} \\
&= \int_0^\infty{e^{-(a+j\omega) t}\text{d}t} \\
&= \left. \frac{e^{-(a+j\omega)t}}{-(a+j\omega)} \right|^\infty_0 \\
&= \frac{1}{a+j\omega}
\end{align}
$$

## 2 ##

求 $ f(t) = \left\{ \begin{align}  &t    & 0 \leq t \lt \tau \\    &\tau & \tau \leq t \lt 2\tau \\    &0    & other \end{align} \right.$ 的傅里叶变换. 

$$
\begin{align}
F(j\omega) &= \mathcal{F}[f(t)] \\
&= \int_{-\infty}^{+\infty}{f(t)e^{-j\omega t}\text{d}t} \\
&= \int_0^\tau{te^{-j\omega t}\text{d}t} + \int_\tau^{2\tau}{\tau e^{-j\omega t}\text{d}t} \\
&= \frac{j\omega \tau + 1}{\omega^2}e^{-j\omega \tau}-\frac{1}{\omega^2} + \frac{j\tau}{\omega}(e^{-j\omega \tau}-1)e^{-j\omega\tau} \\ 
&= -\frac{1}{(j\omega)^2}e^{-\tau j\omega} - \frac{\tau}{j\omega}e^{-2\tau j\omega}+\frac{1}{(j\omega)^2}
\end{align}
$$

