# 信号处理原理 第 9 次作业 #

李祥泽 2018011331

------

由题意
$$
e^{-j(n+N)\omega_k}=e^{-jn\omega_k} \cdot e^{-jN\frac{k\cdot2\pi}{N}}=e^{-jn\omega_k}
$$
那么, 欲证等式的右边可如下变换: $\forall k =0,1,2,3,\dots,N-1$
$$
\begin{align}
&\quad \sum_{n=0}^{L-1}{x(n)e^{-jn\omega_k}} \\
&= \sum_{n=0}^{N-1}{x(n)e^{-jn\omega_k}}+\sum_{n=N}^{2N-1}{x(n)e^{-jn\omega_k}}+\dots+\sum_{n=rN}^{L-1}{x(n)e^{-jn\omega_k}} \\
&= \sum_{n=0}^{N-1}{x(n)e^{-jn\omega_k}}+\sum_{n=0}^{N-1}{x(n+N)e^{-j(n+N)\omega_k}}+\dots+\sum_{n=0}^{s-1}{x(n+rN)e^{-jn\omega_k}} \\
&\text{由于序列最后部分补零, 即 }x(n)=0,\ n=L,L+1,\dots,N-1+rN \\
&= \sum_{n=0}^{N-1}{x(n)e^{-jn\omega_k}}+\sum_{n=0}^{N-1}{x(n+N)e^{-jn\omega_k}}+\dots+\sum_{n=0}^{N-1}{x(n+rN)e^{-jn\omega_k}} \\
&= \sum_{n=0}^{N-1}{\left[\sum_{m=0}^{r-1}{x(n+mN)}\right]e^{-jn\omega_k}} \\
&= \sum_{n=0}^{N-1}{\tilde x(n)e^{-jn\omega_k}}=\text{等式右边}
\end{align}
$$

即证. 